Prove dlo_atom and dlo_atomeq

atom.lean
@@ -1,14 +1,14 @@
 import .logic
 
 class atom (α β : Type) :=
-(I_a : α → list β → Prop)
+(val : α → list β → Prop)
 (aneg : α → fm α) 
 (aneg_nqfree : ∀ (a : α), nqfree (aneg a))
-(aneg_prsv : ∀ (a : α) (xs : list β), (interp I_a xs (aneg a)) = (interp I_a xs (¬' A' a)))
+(aneg_prsv : ∀ (a : α) (xs : list β), (interp val xs (aneg a)) = (interp val xs (¬' A' a)))
 (dep0 : α → Prop)
 (dec_dep0 : decidable_pred dep0)
 (decr : α → α)
-(decr_prsv : ∀ (a : α), ¬ (dep0 a) → ∀ (b : β) (bs : list β), (I_a (decr a) bs = I_a a (b::bs)))
+(decr_prsv : ∀ (a : α), ¬ (dep0 a) → ∀ (b : β) (bs : list β), (val (decr a) bs = val a (b::bs)))
 (inh : β)
 (dec_eq : decidable_eq α)
 
@@ -16,25 +16,30 @@ class atomeq (α β : Type) extends atom α β :=
 (solv0 : α → Prop)
 (dec_solv0 : decidable_pred solv0)
 (dest_solv0 : ∀ a, solv0 a → nat)
-(solv0_eq : ∀ {e : α} (He : solv0 e) {b} {bs}, I_a e (b::bs) 
+(solv0_eq : ∀ {e : α} (He : solv0 e) {b} {bs}, val e (b::bs) 
   → list.nth_dft (atom.inh α β) (b::bs) (dest_solv0 e He) = b)
 (trivial : α → Prop)
 (dec_triv : decidable_pred trivial)
-(true_triv : ∀ a, trivial a → ∀ xs, I_a a xs)
+(true_triv : ∀ a, trivial a → ∀ xs, val a xs)
 (subst0 : α → α → α)
-(true_subst : ∀ e, solv0 e → ∀ bs, I_a (subst0 e e) bs)
+(true_subst : ∀ e, solv0 e → ∀ bs, val (subst0 e e) bs)
 (subst_prsv : ∀ {e : α} (He : solv0 e), ∀ {a : α} {bs : list β}, 
-  I_a (subst0 e a) bs ↔ I_a a ((list.nth_dft (atom.inh α β) bs (dest_solv0 e He - 1))::bs))
+  val (subst0 e a) bs ↔ val a ((list.nth_dft (atom.inh α β) bs (dest_solv0 e He - 1))::bs))
 (dest_pos : ∀ {a} {Ha : solv0 a}, ¬ trivial a → dest_solv0 a Ha > 0)
 
+-- Requires : j = 0 ↔ ¬(i = 0)
 def subst_idx : nat → nat → nat → nat 
 | 0 j 0 := j - 1
-| i j 0 := i - 1 
-| _ _ k := k - 1
+| (i+1) _ 0 := i  
+| _ _ k := k - 1 
+
+-- Qstn : Why do I need this? (Why doesn't unfold work?)
+lemma exp_subst_idx_i0 (i) : subst_idx (i+1) 0 0 = i := 
+begin refl end
 
 variables {α β : Type}
 
-def I [atom α β] (p : fm α) (xs : list β) := interp (atom.I_a) xs p 
+def I [atom α β] (p : fm α) (xs : list β) := interp (atom.val) xs p 
 
 lemma exp_I_and [atom α β] (p q : fm α) (xs : list β) : 
   I (p ∧' q) xs = ((I p xs) ∧ (I q xs)) := eq.refl _
