dlo.lean
@@ -1,4 +1,4 @@
-import .lnf
+import .ldeq
 
 variables {α β : Type}
 
@@ -17,9 +17,9 @@ inductive adlo : Type
 notation x `<'` y := adlo.lt x y 
 notation x `='` y := adlo.eq x y 
 
-def I_adlo [dlo β] : adlo → list β → Prop 
-| (adlo.lt m n) l := (nth_def (inh _) l m) < (nth_def (inh _) l n) 
-| (adlo.eq m n) l := (nth_def (inh _) l m) = (nth_def (inh _) l n) 
+def dlo_val [dlo β] : adlo → list β → Prop 
+| (adlo.lt m n) l := (list.nth_dft (inh _) l m) < (list.nth_dft (inh _) l n) 
+| (adlo.eq m n) l := (list.nth_dft (inh _) l m) = (list.nth_dft (inh _) l n) 
 
 def adlo_aneg : adlo → fm adlo
 | (adlo.lt m n) := (A' (adlo.eq m n)) ∨' (A' (adlo.lt n m))
@@ -30,11 +30,11 @@ lemma adlo_aneg_nqfree : ∀ (d : adlo), nqfree (adlo_aneg d)
 | (adlo.eq m n) := and.intro trivial trivial
 
 lemma adlo_aneg_prsv [dlo β] : ∀ (d : adlo) (l : list β), 
-  interp I_adlo l (adlo_aneg d) = interp I_adlo l (¬' A' d) 
+  interp dlo_val l (adlo_aneg d) = interp dlo_val l (¬' A' d) 
 | (adlo.lt m n) l := 
   begin
     unfold adlo_aneg, unfold interp, 
-    unfold I_adlo, apply propext, 
+    unfold dlo_val, apply propext, 
     apply iff.intro, 
     intro H, apply not_lt_of_ge,
     apply le_of_lt_or_eq, 
@@ -45,7 +45,7 @@ lemma adlo_aneg_prsv [dlo β] : ∀ (d : adlo) (l : list β),
   end
 | (adlo.eq m n) l := 
   begin
-    unfold adlo_aneg, unfold interp, unfold I_adlo,
+    unfold adlo_aneg, unfold interp, unfold dlo_val,
     apply propext, apply iff.intro, 
     intro H, cases H with H H, 
     apply ne_of_lt H, apply ne_of_gt H, 
@@ -56,42 +56,258 @@ def dlo_dep0 : adlo → Prop
 | (adlo.lt m n) := m = 0 ∨ n = 0
 | (adlo.eq m n) := m = 0 ∨ n = 0
 
+lemma adlo_dec_dep0 : decidable_pred dlo_dep0  
+| (adlo.lt 0 n) := decidable.is_true (or.inl (eq.refl _))
+| (adlo.lt m 0) := decidable.is_true (or.inr (eq.refl _))
+| (adlo.lt (m+1) (n+1)) := 
+ decidable.is_false 
+  (begin 
+    intro H, cases H with H H,
+    cases H, cases H
+   end)
+| (adlo.eq 0 n) := decidable.is_true (or.inl (eq.refl _))
+| (adlo.eq m 0) := decidable.is_true (or.inr (eq.refl _))
+| (adlo.eq (m+1) (n+1)) := 
+ decidable.is_false 
+  (begin 
+    intro H, cases H with H H,
+    cases H, cases H
+   end)
+
 def dlo_decr : adlo → adlo
 | (adlo.lt m n) := (adlo.lt (m-1) (n-1))
 | (adlo.eq m n) := (adlo.eq (m-1) (n-1))
 
-theorem atom_adlo [dlo β] : atom adlo β := 
-{ I_a := I_adlo,
+def pos_of_not_dep0_lt (m n) (H : ¬ dlo_dep0 (m <' n)) : (m > 0 ∧ n > 0) := 
+begin
+  cases m, apply absurd _ H, 
+  apply or.inl, refl, 
+  cases n, apply absurd _ H, 
+  apply or.inr, refl, 
+  apply and.intro, 
+  apply nat.zero_lt_succ,
+  apply nat.zero_lt_succ,
+end
+
+def pos_of_not_dep0_eq (m n) (H : ¬ dlo_dep0 (m =' n)) : (m > 0 ∧ n > 0) := 
+begin
+  cases m, apply absurd _ H, 
+  apply or.inl, refl, 
+  cases n, apply absurd _ H, 
+  apply or.inr, refl, 
+  apply and.intro, 
+  apply nat.zero_lt_succ,
+  apply nat.zero_lt_succ,
+end
+
+theorem dlo_atom [dlo β] : atom adlo β := 
+{ val := dlo_val,
   aneg := adlo_aneg,
   aneg_nqfree := adlo_aneg_nqfree,
   aneg_prsv := adlo_aneg_prsv,
   dep0 := dlo_dep0,
-  decr := dlo_decr } 
+  dec_dep0 := adlo_dec_dep0,
+  decr := dlo_decr,
+  decr_prsv := 
+    begin
+      intros a Ha b bs, 
+      cases a with m n m n, 
+      unfold dlo_decr, 
+      repeat {unfold dlo_val}, 
+      repeat {rewrite nth_dft_pred}, 
+      apply (pos_of_not_dep0_lt m n Ha)^.elim_right,
+      apply (pos_of_not_dep0_lt m n Ha)^.elim_left,
+      unfold dlo_decr, 
+      repeat {unfold dlo_val}, 
+      repeat {rewrite nth_dft_pred}, 
+      repeat {rewrite nth_dft_pred}, 
+      apply (pos_of_not_dep0_eq m n Ha)^.elim_right,
+      apply (pos_of_not_dep0_eq m n Ha)^.elim_left,
+    end,
+  inh := dlo.inh β,
+  dec_eq := by tactic.mk_dec_eq_instance } 
 
-def dlo_sovable0 : adlo → Prop  
+def dlo_solv0 : adlo → Prop  
 | (adlo.lt m n) := false
 | (adlo.eq m n) := m = 0 ∨ n = 0 
 
-def dlo_trivial : adlo → Prop  
+lemma dlo_dec_solv0 : decidable_pred dlo_solv0 
+| (adlo.lt m n) := is_false (λ H, by cases H)
+| (adlo.eq m n) := 
+  begin
+    cases m with m m, apply is_true, apply or.inl, refl,
+    cases n with n n, apply is_true, apply or.inr, refl,
+    apply is_false, intro H, cases H with H H,
+    cases H, cases H 
+  end
+
+def dlo_dest_solv0 : ∀ (a : adlo) (H : dlo_solv0 a), nat 
+| (adlo.lt m n) H := by cases H
+| (adlo.eq 0 n) _ := n
+| (adlo.eq (m+1) 0) _ := m+1
+| (adlo.eq (m+1) (n+1)) H := 
+  begin exfalso, cases H with H H; cases H end
+
+lemma exp_dlo_dest_solv0_0n (n : nat) (H : dlo_solv0 (0 ='n)) : 
+  dlo_dest_solv0 (0 =' n) H = n := by refl 
+
+lemma exp_dlo_dest_solv0_m0 (m : nat) (H : dlo_solv0 ((m+1) =' 0)) : 
+  dlo_dest_solv0 ((m+1) =' 0) H = m+1 := by refl
+
+lemma dlo_solv0_eq [dlo β] : ∀ {e : adlo} (He : dlo_solv0 e) {b} {bs}, dlo_val e (b::bs) 
+  → list.nth_dft (dlo.inh β) (b::bs) (dlo_dest_solv0 e He) = b   
+| (adlo.lt m n) He _ _ _ := by cases He
+| (adlo.eq 0 n) He b bs HI := 
+  begin
+    cases n; unfold dlo_dest_solv0, refl, 
+    unfold dlo_val at HI, apply eq.symm HI
+  end
+| (adlo.eq m 0) He b bs HI := 
+  begin
+    cases m with m; unfold dlo_dest_solv0, refl, 
+    unfold dlo_val at HI, apply HI
+  end
+| (adlo.eq (m+1) (n+1)) He _ _ _ := 
+  begin cases He with He He; cases He end
+
+def dlo_triv : adlo → Prop  
 | (adlo.lt m n) := false
 | (adlo.eq m n) := m = n
 
-def dlo_subst0 : nat → nat → adlo → adlo
-| i j (m <' n) := subst_idx i j m <' subst_idx i j n
-| i j (m =' n) := subst_idx i j m =' subst_idx i j n
+lemma dlo_dec_triv : decidable_pred dlo_triv
+| (adlo.lt m n) := begin apply is_false, apply id end
+| (adlo.eq m n) := 
+  begin
+    cases (nat.decidable_eq m n) with HD HD, 
+    apply is_false, intro HC, apply HD HC, 
+    apply is_true, apply HD
+  end
 
-theorem atomeq_adlo [dlo β] : atomeq adlo β := 
-{ I_a := I_adlo,
+lemma dlo_true_triv [dlo β] : ∀ a, dlo_triv a → ∀ (bs : list β), dlo_val a bs 
+| (adlo.lt m n) HT := by cases HT 
+| (adlo.eq m n) HT := 
+  begin 
+    intro bs, unfold dlo_triv at HT, 
+    rewrite HT, unfold dlo_val 
+  end
+
+def dlo_subst0 : adlo → adlo → adlo
+| (i =' j) (m <' n) := subst_idx i j m <' subst_idx i j n
+| (i =' j) (m =' n) := subst_idx i j m =' subst_idx i j n
+| _        a        := a
+
+lemma dlo_true_subst [dlo β] : ∀ e, dlo_solv0 e 
+  → ∀ (bs : list β), dlo_val (dlo_subst0 e e) bs  
+| (adlo.lt m n) HT := by cases HT 
+| (adlo.eq m n) HT := 
+  begin 
+    intro bs, cases HT with HT HT, 
+    subst HT, unfold dlo_subst0, 
+    cases n with n, 
+    repeat {unfold subst_idx},
+    unfold dlo_val, 
+    repeat {unfold subst_idx},
+    unfold dlo_val, refl,
+    rewrite HT, unfold dlo_subst0, 
+    cases m with m, unfold dlo_val, 
+    repeat {unfold subst_idx}, 
+    unfold dlo_val, refl
+  end
+
+lemma dlo_subst_prsv_aux_0n [dlo β] (n x) (bs) (H) : list.nth_dft (inh β) bs (subst_idx 0 n x) 
+  = list.nth_dft (inh β) (list.nth_dft (inh β) bs (dlo_dest_solv0 (0 =' n) H - 1) :: bs) x := 
+begin
+  cases x with x, unfold subst_idx,
+  rewrite exp_dlo_dest_solv0_0n, 
+  rewrite nth_dft_head, refl
+end
+
+lemma dlo_subst_prsv_aux_m0 [dlo β] (m x) (bs) (H) : list.nth_dft (inh β) bs (subst_idx m 0 x) 
+  = list.nth_dft (inh β) (list.nth_dft (inh β) bs (dlo_dest_solv0 (m =' 0) H - 1) :: bs) x := 
+begin
+  cases m with m, apply dlo_subst_prsv_aux_0n,
+  cases x with x, unfold subst_idx,
+  rewrite exp_dlo_dest_solv0_m0, 
+  rewrite nth_dft_head, refl, refl
+end
+
+lemma dlo_subst_prsv [dlo β] : ∀ {e : adlo} (He : dlo_solv0 e) {a : adlo} {bs : list β}, 
+  dlo_val (dlo_subst0 e a) bs ↔ dlo_val a ((list.nth_dft (dlo.inh β) bs (dlo_dest_solv0 e He - 1))::bs) 
+| (adlo.lt m n) H _ := by cases H
+| (adlo.eq 0 n) _ (x <' y) := 
+  begin
+    intro bs, unfold dlo_subst0,
+    repeat {unfold dlo_val},  
+    repeat {rewrite dlo_subst_prsv_aux_0n}
+  end
+| (adlo.eq 0 n) _ (x =' y) :=
+  begin
+    intro bs, unfold dlo_subst0,
+    repeat {unfold dlo_val},  
+    repeat {rewrite dlo_subst_prsv_aux_0n}
+  end
+| (adlo.eq m 0) _ (x <' y) := 
+  begin
+    intro bs, unfold dlo_subst0,
+    repeat {unfold dlo_val},  
+    repeat {rewrite dlo_subst_prsv_aux_m0}
+  end
+| (adlo.eq m 0) _ (x =' y) := 
+  begin
+    intro bs, unfold dlo_subst0,
+    repeat {unfold dlo_val},  
+    repeat {rewrite dlo_subst_prsv_aux_m0}
+  end
+| (adlo.eq (m+1) (n+1)) H _ := by cases H with H H ; cases H
+
+lemma dlo_dest_pos : ∀ {a} {Ha : dlo_solv0 a}, ¬ dlo_triv a → dlo_dest_solv0 a Ha > 0 :=
+begin
+  intros a Ha HT, cases a with m n m n, 
+  cases Ha, cases m ; cases n, 
+  exfalso, apply HT, unfold dlo_triv, 
+  unfold dlo_dest_solv0, apply nat.zero_lt_succ,
+  unfold dlo_dest_solv0, apply nat.zero_lt_succ,
+  unfold dlo_solv0 at Ha, cases Ha with Ha Ha ; 
+  cases Ha
+end
+
+lemma dlo_atomeq [H : dlo β] : atomeq adlo β := 
+{ val := dlo_val,
   aneg := adlo_aneg,
   aneg_nqfree := adlo_aneg_nqfree,
   aneg_prsv := adlo_aneg_prsv,
   dep0 := dlo_dep0,
+  dec_dep0 := adlo_dec_dep0,
   decr := dlo_decr,
-  solv0 := dlo_sovable0,
-  trivial := dlo_trivial,
-  subst0 := dlo_subst0 } 
-
-#exit
+  decr_prsv := 
+    begin
+      intros a Ha b bs, 
+      cases a with m n m n, 
+      unfold dlo_decr, 
+      repeat {unfold dlo_val}, 
+      repeat {rewrite nth_dft_pred}, 
+      apply (pos_of_not_dep0_lt m n Ha)^.elim_right,
+      apply (pos_of_not_dep0_lt m n Ha)^.elim_left,
+      unfold dlo_decr, 
+      repeat {unfold dlo_val}, 
+      repeat {rewrite nth_dft_pred}, 
+      repeat {rewrite nth_dft_pred}, 
+      apply (pos_of_not_dep0_eq m n Ha)^.elim_right,
+      apply (pos_of_not_dep0_eq m n Ha)^.elim_left,
+    end,
+  inh := dlo.inh β,
+  dec_eq := by tactic.mk_dec_eq_instance, 
+  solv0 := dlo_solv0,
+  dec_solv0 := dlo_dec_solv0,
+  dest_solv0 := dlo_dest_solv0,
+  solv0_eq := @dlo_solv0_eq β _, 
+  trivial := dlo_triv,
+  dec_triv := dlo_dec_triv,  
+  true_triv := dlo_true_triv,
+  subst0 := dlo_subst0,
+  true_subst := dlo_true_subst,
+  subst_prsv := @dlo_subst_prsv β _,
+  dest_pos := @dlo_dest_pos }
 
 def lt_has_0 : adlo → Prop 
 | (adlo.eq _ _) := false
@@ -106,17 +322,24 @@ def lt_single_0 : adlo → Prop
 | (adlo.lt 0 _) := true
 | (adlo.lt (i+1) (j+1)) := false
 
-def qe_dlo_aux : ∀ (l : list adlo) (H : allp l lt_single_0), (list nat × list nat)
+def qe_dlo_aux : ∀ (l : list adlo) (H : allp lt_single_0 l), (list nat × list nat)
 | [] := λ _, ([],[]) 
 | (a::as) :=
   match a with 
-  | (adlo.eq _ _) := begin intro H, exfalso, apply H^.elim_left end
-  | (adlo.lt 0 0) := begin intro H, exfalso, apply H^.elim_left end
-  | (adlo.lt (i+1) 0) := λ H, let (lbs,rbs) := qe_dlo_aux as (H^.elim_right) in (i::lbs,rbs)
-  | (adlo.lt 0 (j+1)) := λ H, let (lbs,rbs) := qe_dlo_aux as (H^.elim_right) in (lbs,j::rbs)
-  | (adlo.lt (i+1) (j+1)) := begin intro H, exfalso, apply H^.elim_left end
+  | (adlo.eq m n) := begin intro H, exfalso, apply H _ (or.inl (eq.refl _)) end
+  | (adlo.lt 0 0) := begin intro H, exfalso, apply H _ (or.inl (eq.refl _)) end
+  | (adlo.lt (i+1) 0) := 
+    λ H, let (lbs,rbs) := qe_dlo_aux as 
+      (begin intros a' Ha', apply H a' (or.inr Ha') end) in 
+      (i::lbs,rbs)
+  | (adlo.lt 0 (j+1)) := 
+    λ H, let (lbs,rbs) := qe_dlo_aux as 
+      (begin intros a' Ha', apply H a' (or.inr Ha') end) in 
+      (lbs,j::rbs)
+  | (adlo.lt (i+1) (j+1)) := begin intro H, exfalso, apply H _ (or.inl (eq.refl _)) end
   end
 
+#exit
 lemma allp_single_0_of : ∀ (as : list adlo) (H : allp as lt_has_0) (HZ : (0 <' 0) ∉ as), allp as lt_single_0  
 | [] _ _ := trivial 
 | ((adlo.eq _ _)::as) H HZ := 
